theories/TRAKHTENBROT/fo_sat.v
@@ -12,6 +12,9 @@ Require Import List.
 From Undecidability.Shared.Libs.DLW.Utils
   Require Import finite.
 
+From Undecidability.Shared.Libs.DLW.Vec
+  Require Import pos vec.
+
 From Undecidability.TRAKHTENBROT
   Require Import notations fol_ops fo_terms fo_logic.
 
@@ -19,7 +22,7 @@ Set Implicit Arguments.
 
 Section satisfiability.
 
-  Variable (Σ : fo_signature) (A : fol_form Σ).
+  Variable (Σ : fo_signature) (e : rels Σ) (A : fol_form Σ).
 
   (** A first order formula over signature Σ is finitely satisfiable over
       type X if there exists a model M interpreting the signature Σ over type X
@@ -39,12 +42,22 @@ Section satisfiability.
            (φ : nat -> X), 
            fol_sem M φ A.
 
+  Definition fo_form_fin_dec_eq_SAT_in X := 
+    exists (M : fo_model Σ X)  
+           (_ : finite_t X) 
+           (_ : fo_model_dec M)
+           (E : ar_rels Σ e = 2) 
+           (_ : eq_rect _ (fun n => vec _ n -> _) (fom_rels M e) _ E = rel2_on_vec eq)
+           (φ : nat -> X), 
+           fol_sem M φ A.
+
   Definition fo_form_fin_discr_dec_SAT_in X := 
     exists (_ : discrete X), 
            fo_form_fin_dec_SAT_in X.
 
   Definition fo_form_fin_SAT := ex fo_form_fin_SAT_in.
   Definition fo_form_fin_dec_SAT := ex fo_form_fin_dec_SAT_in.
+  Definition fo_form_fin_dec_eq_SAT := ex fo_form_fin_dec_eq_SAT_in.
   Definition fo_form_fin_discr_dec_SAT := ex fo_form_fin_discr_dec_SAT_in.
 
   Fact fo_form_fin_discr_dec_SAT_fin_dec : fo_form_fin_discr_dec_SAT -> fo_form_fin_dec_SAT.
