theories/TRAKHTENBROT/reductions.v
@@ -21,10 +21,15 @@ From Undecidability.Shared.Libs.DLW.Wf
   Require Import wf_finite.
 
 From Undecidability.TRAKHTENBROT
-  Require Import notations fol_ops fo_terms fo_logic fo_sat discrete Sig3_Sig2 
-                 bpcp fol_bpcp.
+  Require Import notations fol_ops fo_terms fo_logic fo_sat discrete 
+                 Sig3_Sig2 Sig32_Sig2 bpcp fol_bpcp.
 
 Set Implicit Arguments.
+
+(** The reduction from PBCP to SAT of a FO formula 
+     - over signature Σbpcp (2 unary funs, 2 constants, 3 rels)
+     - within finite and decidable models
+  *)
 
 Section BPCP_fo_fin_dec_SAT.
 
@@ -46,7 +51,12 @@ End BPCP_fo_fin_dec_SAT.
 Check BPCP_FIN_DEC_SAT.
 Print Assumptions BPCP_FIN_DEC_SAT.
 
-(** The reduction is the identity here !! *)
+(** From a given (arbitrary) signature, 
+    the reduction from 
+    - finite and decidable SAT  
+    - to finite and decidable and discrete SAT
+
+    The reduction is the identity here !! *)
 
 Theorem fo_form_fin_dec_SAT_discr_equiv Σ A : 
     @fo_form_fin_dec_SAT Σ A <-> @fo_form_fin_discr_dec_SAT Σ A.
@@ -64,9 +74,13 @@ Proof. exists (fun A => A); apply fo_form_fin_dec_SAT_discr_equiv. Qed.
 Check FIN_DEC_SAT_FIN_DISCR_DEC_SAT.
 Print Assumptions FIN_DEC_SAT_FIN_DISCR_DEC_SAT.
 
-Print Σrel.
+(** With Σrel 3 signature with a unique ternary symbol
+     and Σrel 2 signature with a unique binary symbol
+   the reduction from 
+   - finite and decidable and discrete SAT over Σrel 3
+   - to finite and decidable SAT over Σrel 2 *)
 
-Theorem FIN_DISCR_DEC_3SAT_FIN_DEC_SAT : @fo_form_fin_discr_dec_SAT (Σrel 3)
+Theorem FIN_DISCR_DEC_3SAT_FIN_DEC_2SAT : @fo_form_fin_discr_dec_SAT (Σrel 3)
                                                                         ⪯ @fo_form_fin_dec_SAT (Σrel 2).
 Proof.
   exists Σ3_Σ2_enc; intros A; split.
@@ -74,5 +88,24 @@ Proof.
   + intros H; apply fo_form_fin_dec_SAT_fin_discr_dec, SAT2_SAT3, H.
 Qed.
 
-Check FIN_DISCR_DEC_3SAT_FIN_DEC_SAT.
-Print Assumptions FIN_DISCR_DEC_3SAT_FIN_DEC_SAT.
+Check FIN_DISCR_DEC_3SAT_FIN_DEC_2SAT.
+Print Assumptions FIN_DISCR_DEC_3SAT_FIN_DEC_2SAT.
+
+(** With Σrel_eq 3 signature with a ternary symbol AND an interpret equality
+     and Σrel 2 signature with a unique binary symbol
+   the reduction from 
+   - finite and decidable and interpreted equality SAT over Σrel_eq 3 
+   - to finite and decidable SAT over Σrel 2 *)
+
+Print Σrel_eq.
+
+Theorem FIN_DEC_EQ_3SAT_FIN_DEC_2SAT : @fo_form_fin_dec_eq_SAT (Σrel_eq 3) false
+                                                                      ⪯ @fo_form_fin_dec_SAT (Σrel 2).
+Proof.
+  exists Σ3eq_Σ2_enc; intros A; split.
+  + apply SAT32_SAT2.
+  + apply SAT2_SAT32.
+Qed.
+
+Check FIN_DEC_EQ_3SAT_FIN_DEC_2SAT.
+Print Assumptions FIN_DEC_EQ_3SAT_FIN_DEC_2SAT.
